src/coq/Handlers/Memory.v
@@ -117,12 +117,22 @@ Module Addr : MemoryAddress.ADDRESS with Definition addr := (Z * Z) % type.
   Qed.
 End Addr.
 
+Module Mem : MemoryAddress.MEMORYSTATE with Definition memory := unit.
+  Definition memory := unit.
+  Lemma eq_dec : forall (a b : unit), {a = b} + {a <> b}.
+  Proof.
+    intros a b.
+    destruct a. destruct b.
+    left. reflexivity.
+  Qed.
+End Mem.
+
 (** ** Memory model
     Implementation of the memory model, i.e. a handler for [MemoryE].
     The memory itself, [memory], is a finite map (using the standard library's AVLs)
     indexed on [Z].
  *)
-Module Make(LLVMEvents: LLVM_INTERACTIONS(Addr)).
+Module Make(LLVMEvents: LLVM_INTERACTIONS(Addr)(Mem)).
   Import LLVMEvents.
   Import DV.
   Open Scope list.
@@ -1093,11 +1103,11 @@ Module Make(LLVMEvents: LLVM_INTERACTIONS(Addr)).
 
       | Alloca t =>
         '(m',a) <- lift_pure_err (allocate m t);;
-        ret (m', DVALUE_Addr a)
+        ret (m', UVALUE_Addr a)
 
       | Load t uv =>
-        match dv with
-        | DVALUE_Addr ptr =>
+        match uv with
+        | UVALUE_Addr ptr =>
           match read m ptr t with
           | inr v => ret (m, v)
           | inl s => raiseUB s
